theories/prob_eff_lang/probblaze/examples/DH_KE/dhke_channel_lazy_real_one.v
@@ -44,15 +44,15 @@ Section handlee_verification.
     (∀ᵣ θₕ, ((sem_ty_sum 𝟙 𝟙) -{ θₕ }-> (Option 𝔾)) -{ sem_row_union θₕ L }-∘ 𝟙)%T f1 f2 -∗
 
     BREL DH_KE f1 ≤ C_lazy DH_real f2 <|⊥|> {{ λ v1 v2, 
-                                                 ∀ c1 c2 : label, let ac := authchan_rowL c1 c2 γtoka atokN γtokb btokN γfraca γfracb γautha γauthb in
-                                                                  BREL v1 ((λ: "m", do: c1 (Send "m")), (λ: "m", do: c1 (Recv "m")))%V ≤
-                                                                    v2 ((λ: "m", do: c2 (Send "m")), (λ: "m", do: c2 (Recv "m")))%V 
+                                                 ∀ send1 send2 recv1 recv2 : label, let ac := chan_rowL send1 send2 recv1 recv2 γtoka atokN γtokb btokN γfraca γfracb γautha γauthb in
+                                                                  BREL v1 ((λ: "m", do: send1 "m"), (λ: "m", do: recv1 "m"))%V ≤
+                                                                    v2 ((λ: "m", do: send2 "m"), (λ: "m", do: recv2 "m"))%V 
                                                                     <| (iLblSig_to_iLblThy ac) ++ (iLblSig_to_iLblThy L) |> {{ (λ w1 w2, 𝟙%T w1 w2) }} }}.
   Proof with (repeat foldkont) using G.
     iIntros "Htoka Htokb Ha Hb Hff". 
     unfold DH_KE, C_lazy. 
     brel_pures'. iModIntro. 
-    iIntros (c1 c2). set (ac := authchan_rowL c1 c2 γtoka atokN γtokb btokN γfraca γfracb γautha γauthb).
+    iIntros (send1 send2 recv1 recv2). set (ac := chan_rowL send1 send2 recv1 recv2 γtoka atokN γtokb btokN γfraca γfracb γautha γauthb).
     brel_pures'.
     repeat simpl.
     unfold DH_real. brel_pures'.
@@ -132,7 +132,7 @@ Section handlee_verification.
     iApply (brel_add_label_r with "Hgk2").
     
     iDestruct (brel_introduction_mono _ ([([gk1],[gk2],GetKey gk1 gk2)] ++ (iLblSig_to_iLblThy ac) ++ (iLblSig_to_iLblThy L)) with "[][$Hff]") as "Hf".
-    { iApply to_iThy_le_intro'. apply submseteq_skip. by apply submseteq_cons. }
+    { iApply to_iThy_le_intro'. apply submseteq_skip. by do 2 apply submseteq_cons. }
     iApply (brel_exhaustion with "[$]"); [done|done|].
     
     (* getKey can be called multiple times, why we need induction *)
@@ -173,12 +173,12 @@ Section handlee_verification.
         iSplitL; [iNext; iRight; iFrame "#"|].
         
         iApply (brel_bind' [_] [_]); [iApply traversable_to_iThy|].
-        iApply (brel_introduction' [c1] [c2]).
-        { apply elem_of_cons. right. apply list_elem_of_here. }
+        iApply (brel_introduction' [send1] [send2]).
+        { apply elem_of_cons. right. apply elem_of_cons. right. apply list_elem_of_here. }
         
         iExists _, _, [], [], _. do 2 (iSplit; [done|]; iSplit; [iPureIntro; apply _|]).
         iSplitL; [|by iIntros "!>" (??) "H"; iApply "H"].
-        iLeft. iLeft. iExists _,_,_.
+        iLeft. iExists _,_,_.
         iSplitL.
         { iMod (inv_acc with "Hinvta") as "([>Htok | >#Hfrac'] & Hclose)"; try done.
           - iModIntro. iLeft.
@@ -193,11 +193,11 @@ Section handlee_verification.
         brel_pures'.
         
         iApply (brel_bind' [_] [_]); [iApply traversable_to_iThy|].
-        iApply (brel_introduction' [c1] [c2]).
+        iApply (brel_introduction' [recv1] [recv2]).
         { apply elem_of_cons. right. apply list_elem_of_here. }
         iExists _, _, [], [], _. do 2 (iSplit; [done|]; iSplit; [iPureIntro; apply _|]).
         iSplitL; [|by iIntros "!>" (??) "H"; iApply "H"].
-        iLeft. iRight.
+        iRight.
         do 2 (iSplit; try (iPureIntro; done)).
         iModIntro.
         iSplitL.
@@ -226,11 +226,11 @@ Section handlee_verification.
         iApply (brel_load_r with "Hlcs"). iIntros "_". brel_pures'.
         
         iApply (brel_bind' [_] [_]); [iApply traversable_to_iThy|].
-        iApply (brel_introduction' [c1] [c2]).
-        { apply elem_of_cons. right. apply list_elem_of_here. }
+        iApply (brel_introduction' [send1] [send2]).
+        { apply elem_of_cons. right. apply elem_of_cons. right. apply list_elem_of_here. }
         iExists _, _, [], [], _. do 2 (iSplit; [done|]; iSplit; [iPureIntro; apply _|]).
         iSplitL; [|by iIntros "!>" (??) "H"; iApply "H"].
-        iLeft. iLeft.
+        iLeft.
         iExists _,_,_.
         iSplitL.
         { iMod (inv_acc with "Hinvta") as "([>Htok | >#Hfrac'] & Hclose)"; try done.
@@ -246,11 +246,11 @@ Section handlee_verification.
         brel_pures.
         
         iApply (brel_bind' [_] [_]); [iApply traversable_to_iThy|].
-        iApply (brel_introduction' [c1] [c2]).
+        iApply (brel_introduction' [recv1] [recv2]).
         { apply elem_of_cons. right. apply list_elem_of_here. }
         iExists _, _, [], [], _. do 2 (iSplit; [done|]; iSplit; [iPureIntro; apply _|]).
         iSplitL; [|by iIntros "!>" (??) "H"; iApply "H"].
-        iLeft. iRight.
+        iRight.
         do 2 (iSplit; try (iPureIntro; done)).
         iModIntro.
         iSplitL.
@@ -280,7 +280,7 @@ Section handlee_verification.
       { apply elem_of_cons. right. apply list_elem_of_here. }
       iExists _, _, [], [], _. do 2 (iSplit; [done|]; iSplit; [iPureIntro; apply _|]).
       iSplitL; [|by iIntros "!>" (??) "H"; iApply "H"].
-      iRight. iRight.
+      iLeft.
       do 2 (iSplit; try (iPureIntro; done)).
       iModIntro.
       iSplitL.
@@ -317,10 +317,10 @@ Section handlee_verification.
         iSplitL; [iRight; iFrame "#"|].
         
         iApply (brel_bind' [AppRCtx _] [AppRCtx _]); [iApply traversable_to_iThy|].
-        iApply brel_introduction'. { apply elem_of_cons. right. apply list_elem_of_here. }
+        iApply brel_introduction'. { apply elem_of_cons. right. apply elem_of_cons. right. apply list_elem_of_here. }
         iExists _, _, [], [], _. do 2 (iSplit; [done|]; iSplit; [iPureIntro; apply _|]).
         iSplitL; [|by iIntros "!>" (??) "H"; iApply "H"].
-        iRight. iLeft.
+        iRight.
         iExists _,_.
         iSplitL.
         { iMod (inv_acc with "Hinvtb") as "([>Htok | >#Hfrac'] & Hclose)"; try done.
@@ -353,10 +353,10 @@ Section handlee_verification.
         iApply (brel_load_l with "[$]").
         iIntros "!> _". brel_pures_l. brel_exp_l. brel_pures.
         iApply (brel_bind' [_] [_]); [iApply traversable_to_iThy|].
-        iApply brel_introduction'. { apply elem_of_cons. right. apply list_elem_of_here. }
+        iApply brel_introduction'. { apply elem_of_cons. right. apply elem_of_cons. right. apply list_elem_of_here. }
         iExists _, _, [], [], _. do 2 (iSplit; [done|]; iSplit; [iPureIntro; apply _|]).
         iSplitL; [|by iIntros "!>" (??) "H"; iApply "H"].
-        iRight. iLeft.
+        iRight.
         iExists _,_.
         iSplitL.
         { iMod (inv_acc with "Hinvtb") as "([>Htok | >#Hfrac'] & Hclose)"; try done.
